Get through some crash lock reasoning

src/program_proof/examples/replicated_block_proof.v
@@ -4,6 +4,7 @@ From Perennial.goose_lang Require Import crash_modality.
 From Perennial.algebra Require Import deletable_heap.
 
 From Goose.github_com.mit_pdos.perennial_examples Require Import replicated_block.
+From Perennial.goose_lang.lib Require Import lock.crash_lock.
 From Perennial.program_proof Require Import disk_lib.
 From Perennial.program_proof Require Import proof_prelude.
 
@@ -14,6 +15,8 @@ End rblock.
 Section goose.
   Context `{!heapG Σ}.
   Context `{!lockG Σ}.
+  Context `{!crashG Σ}.
+  Context `{!stagedG Σ}.
 
   Let N := nroot.@"replicated_block".
   Context (P: rblock.t → iProp Σ).
@@ -28,23 +31,32 @@ Section goose.
     ("Hprimary" ∷ int.val addr d↦ σ ∗
      "Hbackup" ∷ ∃ b0, int.val (word.add addr 1) d↦ b0)%I.
 
+  Theorem rblock_linv_to_cinv addr σ :
+    rblock_linv addr σ -∗ rblock_cinv addr σ.
+  Proof.
+    iNamed 1.
+    iFrame "Hprimary".
+    iExists _; iFrame.
+  Qed.
+
   Instance rblock_crash addr σ :
     IntoCrash (rblock_linv addr σ) (λ _, rblock_cinv addr σ).
   Proof.
     rewrite /IntoCrash.
-    iNamed 1.
-    rewrite /rblock_cinv.
-    iFrame "Hprimary".
-    iIntros (???) "?".
-    iExists _; iFrame.
+    rewrite rblock_linv_to_cinv.
+    iIntros "$".
+    auto.
   Qed.
 
-  Definition is_rblock (γ: gname) (l: loc) addr : iProp Σ :=
+  Definition is_rblock (γ: gname) (k': nat) (l: loc) addr : iProp Σ :=
     ∃ (d_ref m_ref: loc),
       "#d" ∷ readonly (l ↦[RepBlock.S :: "d"] #d_ref) ∗
       "#addr" ∷ readonly (l ↦[RepBlock.S :: "addr"] #addr) ∗
       "#m" ∷ readonly (l ↦[RepBlock.S :: "m"] #m_ref) ∗
-      "#Hlock" ∷ is_lock N γ #m_ref (∃ σ, "Hlkinv" ∷ rblock_linv addr σ ∗ "HP" ∷ P σ).
+      "#Hlock" ∷ is_crash_lock N N (LVL k') γ #m_ref (* XXX: what is the nat? *)
+      (∃ σ, "Hlkinv" ∷ rblock_linv addr σ ∗ "HP" ∷ P σ)
+      (∃ σ, "Hclkinv" ∷ rblock_cinv addr σ ∗ "HP" ∷ P σ)
+  .
 
   Definition block0: Block :=
     list_to_vec (replicate (Z.to_nat 4096) (U8 0)).
@@ -59,36 +71,81 @@ Section goose.
     - iExists block0; iExact "Hb".
   Qed.
 
-  Theorem wp_Open (d_ref: loc) addr σ :
+  Theorem wp_Open {k E2} (d_ref: loc) k' addr σ :
+    (k' < S k)%nat →
     {{{ rblock_cinv addr σ ∗ P σ }}}
-      Open #d_ref #addr
-    {{{ γ (l:loc), RET #l; is_rblock γ l addr }}}.
+      Open #d_ref #addr @ NotStuck;LVL (S (S k)); ⊤;E2
+    {{{ γ (l:loc), RET #l; is_rblock γ k' l addr }}}
+    {{{ rblock_cinv addr σ ∗ P σ }}}.
   Proof.
-    iIntros (Φ) "(Hinv&HP) HΦ"; iNamed "Hinv".
-    wp_call.
-    wp_apply (wp_Read with "Hprimary").
+    iIntros (? Φ Φc) "(Hinv&HP) HΦ"; iNamed "Hinv".
+    iDeexHyp "Hbackup".
+    iAssert (□ ∀ b0, int.val addr d↦ σ ∗
+                     int.val (word.add addr 1) d↦ b0 ∗
+                     P σ -∗ rblock_cinv addr σ ∗ P σ)%I
+            as "#Hcrash".
+    { iIntros "!>" (b) "(Hb0&Hb1&HP)".
+      iFrame.
+      iExists _; iFrame. }
+    Ltac prove_crash1 :=
+      iApply ("Hcrash" with "[$]").
+    wpc_call; first by prove_crash1.
+    wpc_apply (wpc_Read with "Hprimary").
+    iSplit; [ | iNext ].
+    { iIntros "Hprimary".
+      crash_case; prove_crash1. }
     iIntros (s) "(Hprimary&Hb)".
     iDestruct (is_slice_to_small with "Hb") as "Hb".
-    wp_apply (wp_Write with "[Hbackup Hb]").
-    { iDeexHyp "Hbackup".
-      iExists _; iFrame. }
+    wpc_pures; first by prove_crash1.
+    wpc_apply (wpc_Write with "[Hbackup Hb]").
+    { iExists _; iFrame. }
+    iSplit; [ | iNext ].
+    { iIntros "Hpost".
+      iDestruct "Hpost" as (b') "(Hbackup&_)".
+      crash_case; prove_crash1. }
     iIntros "(Hbackup&_)".
+
+    (* allocate lock *)
+    wpc_pures; first by prove_crash1.
+    wpc_bind (lock.new _).
+    wpc_frame "HP Hprimary Hbackup HΦ". (* ie, everything *)
+    { crash_case; prove_crash1. }
     wp_apply wp_new_free_lock.
     iIntros (γ m_ref) "Hfree_lock".
-    rewrite -wp_fupd.
+    iNamed 1.
+
+    iApply (alloc_crash_lock N N _ k' _ _ _ _ _ _
+                             (∃ σ, "Hlkinv" ∷ rblock_linv addr σ ∗ "HP" ∷ P σ)%I
+                             (∃ σ, "Hclkinv" ∷ rblock_cinv addr σ ∗ "HP" ∷ P σ)%I
+            with "[$Hfree_lock Hprimary Hbackup HP HΦ]").
+    { lia. }
+    iSplitR.
+    { iIntros "!>"; iNamed 1.
+      iExists _; iFrame.
+      iApply rblock_linv_to_cinv; iFrame. }
+    iSplitL "Hprimary Hbackup HP".
+    { iExists _; iFrame. }
+    iIntros "His_crash_lock".
+
+    (* allocate struct *)
+    rewrite -wpc_fupd.
+    wpc_frame "HΦ".
+    { iNamed 1. crash_case. admit. (* TODO: stuck, crash lock subtracted the
+    crash invariant but this is too weak (it replaced the initial σ with an arbitrary
+    σ') *) }
     wp_apply wp_allocStruct; auto.
     iIntros (l) "Hrb".
+    iNamed 1.
+
+    (* ghost allocation *)
     iDestruct (struct_fields_split with "Hrb") as "(d&addr&m&_)".
-    iMod (alloc_lock N ⊤ _ _ (∃ σ, rblock_linv addr σ ∗ P σ)%I
-            with "Hfree_lock [Hprimary Hbackup HP]") as "Hlock".
-    { iExists _; iFrame. }
     iMod (readonly_alloc_1 with "d") as "d".
     iMod (readonly_alloc_1 with "addr") as "addr".
     iMod (readonly_alloc_1 with "m") as "m".
     iModIntro.
     iApply "HΦ".
     iExists _, _; iFrame.
-  Qed.
+  Admitted.
 
   Theorem wp_RepBlock__readAddr addr l (primary: bool) :
     {{{ readonly (l ↦[RepBlock.S :: "addr"] #addr) }}}
@@ -105,40 +162,80 @@ Section goose.
       iApply "HΦ"; auto.
   Qed.
 
-  Theorem wp_RepBlock__Read (Q: Block → iProp Σ) γ l addr (primary: bool) :
-    {{{ "Hrb" ∷ is_rblock γ l addr ∗
-        "Hfupd" ∷ (∀ σ, P σ ={⊤}=∗ P σ ∗ Q σ) }}}
-      RepBlock__Read #l #primary
-    {{{ s b, RET (slice_val s); is_block s 1 b ∗ Q b }}}.
+  Ltac wpc_bind_seq :=
+    lazymatch goal with
+    | [ |- envs_entails _ (wpc _ _ _ _ (App (Lam _ ?e2) ?e1) _ _) ] =>
+      wpc_bind e1
+    end.
+
+  Theorem wpc_RepBlock__Read (Q: Block → iProp Σ) (Qc: iProp Σ) {k E2} {k' γ l} addr (primary: bool) :
+    (S k < k')%nat →
+    {{{ "Hrb" ∷ is_rblock γ k' l addr ∗
+        "Hfupd" ∷ ((∀ σ, P σ ={⊤ ∖ ↑N}=∗ P σ ∗ Q σ) ∧ Qc) }}}
+      RepBlock__Read #l #primary @ NotStuck; LVL (S (S k)); ⊤; E2
+    {{{ s b, RET (slice_val s); is_block s 1 b ∗ Q b }}}
+    {{{ Qc }}}.
   Proof.
-    iIntros (Φ) "Hpre HΦ"; iNamed "Hpre".
+    iIntros (? Φ Φc) "Hpre HΦ"; iNamed "Hpre".
     iNamed "Hrb".
-    wp_call.
+    Ltac prove_crash1 ::=
+      crash_case; by iRight in "Hfupd".
+    wpc_call; first by prove_crash1.
+    wpc_bind_seq; wpc_frame "HΦ Hfupd"; first by prove_crash1.
     wp_loadField.
-    wp_apply (acquire_spec with "Hlock").
-    iIntros "(His_locked&Hlk)"; iNamed "Hlk".
-    wp_pures.
+    wp_apply (crash_lock.acquire_spec with "Hlock"); auto.
+    iIntros "Hlkd"; iNamed 1.
+    iDestruct "Hlkd" as (γlk) "His_locked".
+    wpc_pures; first by prove_crash1.
+    wpc_bind (RepBlock__readAddr _ _); wpc_frame "HΦ Hfupd"; first by prove_crash1.
     wp_apply (wp_RepBlock__readAddr with "addr").
     iIntros (addr' Haddr'_eq).
+    iNamed 1.
+
+    wpc_bind_seq.
+    iApply (use_crash_locked with "His_locked"); auto.
+    iSplit; first by prove_crash1.
+    iNamed 1.
     iAssert (int.val addr' d↦ σ ∗
                    (int.val addr' d↦ σ -∗ rblock_linv addr σ))%I
       with "[Hlkinv]" as "(Haddr'&Hlkinv)".
     { iNamed "Hlkinv".
       destruct Haddr'_eq; subst; iFrame; auto. }
-    wp_apply (wp_Read with "Haddr'").
+    (* TODO: this isn't what I want, somehow I want to use the right side for
+    the crash condition *)
+    iLeft in "Hfupd".
+    iMod ("Hfupd" with "HP") as "[HP HQ]".
+
+    wpc_apply (wpc_Read with "Haddr'").
+    iSplit; [ | iNext ].
+    { iIntros "Hd".
+      iSpecialize ("Hlkinv" with "Hd").
+      (* iSplitL "HΦ Hfupd"; first by prove_crash1. *)
+      iSplitL "HΦ"; first by admit.
+      iExists _; iFrame.
+      iApply rblock_linv_to_cinv; iFrame. }
     iIntros (s) "(Haddr'&Hb)".
     iDestruct (is_slice_to_small with "Hb") as "Hb".
     iSpecialize ("Hlkinv" with "Haddr'").
-    wp_loadField.
-    iMod ("Hfupd" with "HP") as "[HP HQ]".
-    wp_apply (release_spec with "[$Hlock $His_locked Hlkinv HP]").
+    iSplitR "HP Hlkinv"; last first.
+    (* TODO: why is this the second goal? *)
     { iExists _; iFrame. }
-    wp_pures.
-    iApply "HΦ"; iFrame.
-  Qed.
+    iIntros "His_locked".
+    iSplit; last by admit. (* TODO: why is this the second goal? *)
+    wpc_pures; first by admit.
 
-  Theorem wp_RepBlock__Write (Q: iProp Σ) γ l addr (s: Slice.t) q (b: Block) :
-    {{{ "Hrb" ∷ is_rblock γ l addr ∗
+    wpc_frame "HΦ"; first by admit.
+
+    wp_loadField.
+    wp_apply (crash_lock.release_spec with "[$His_locked]"); auto.
+    wp_pures.
+    iNamed 1.
+    iRight in "HΦ".
+    iApply "HΦ"; iFrame.
+  Admitted.
+
+  Theorem wp_RepBlock__Write (Q: iProp Σ) γ l k' addr (s: Slice.t) q (b: Block) :
+    {{{ "Hrb" ∷ is_rblock γ l k' addr ∗
         "Hb" ∷ is_block s q b ∗
         "Hfupd" ∷ (∀ σ σ', P σ ={⊤}=∗ P σ' ∗ Q) }}}
       RepBlock__Write #l (slice_val s)
@@ -147,6 +244,7 @@ Section goose.
     iIntros (Φ) "Hpre HΦ"; iNamed "Hpre".
     iNamed "Hrb".
     wp_call.
+    (*
     wp_loadField.
     wp_apply (acquire_spec with "Hlock").
     iIntros "(His_locked&Hlk)"; iNamed "Hlk".
@@ -169,5 +267,7 @@ Section goose.
     { iExists _; iFrame. }
     iApply ("HΦ" with "[$]").
   Qed.
+*)
+  Admitted.
 
 End goose.
